Makefile
@@ -46,6 +46,8 @@ COQ_SRCS := $(COQ_DIR)/WpTactics.v \
             $(COQ_DIR)/FindSpec.v \
             $(COQ_DIR)/InsertDefs.v \
             $(COQ_DIR)/InsertSpec.v \
+            $(COQ_DIR)/RebalanceSpec.v \
+            $(COQ_DIR)/InsSpec.v \
             $(COQ_DIR)/RefCount.v \
             $(COQ_DIR)/Invariants.v
 
@@ -111,6 +113,14 @@ $(COQ_DIR)/InsertDefs.vo: $(COQ_DIR)/InsertDefs.v $(COQ_DIR)/RBTree.vo $(COQ_DIR
 $(COQ_DIR)/InsertSpec.vo: $(COQ_DIR)/InsertSpec.v $(COQ_DIR)/RBTree.vo $(COQ_DIR)/TreeRep.vo $(COQ_DIR)/Tactics.vo $(COQ_DIR)/InsertDefs.vo
 	$(COQC) $(COQFLAGS) $<
 
+# Phase 5B: setRebalanceLeft_ok + setRebalanceRight_ok
+$(COQ_DIR)/RebalanceSpec.vo: $(COQ_DIR)/RebalanceSpec.v $(COQ_DIR)/InsertDefs.vo $(COQ_DIR)/Tactics.vo
+	$(COQC) $(COQFLAGS) $<
+
+# Phase 5B: ins_ok (Löb induction, depends on rebalance specs)
+$(COQ_DIR)/InsSpec.vo: $(COQ_DIR)/InsSpec.v $(COQ_DIR)/InsertDefs.vo $(COQ_DIR)/Tactics.vo
+	$(COQC) $(COQFLAGS) $<
+
 $(COQ_DIR)/RefCount.vo: $(COQ_DIR)/RefCount.v $(COQ_DIR)/RBTree.vo $(COQ_DIR)/TreeRep.vo $(COQ_DIR)/Tactics.vo
 	$(COQC) $(COQFLAGS) $<
 
@@ -121,6 +131,7 @@ proofs: $(COQ_DIR)/WpTactics.vo \
         $(COQ_DIR)/RBTree.vo $(COQ_DIR)/TreeRep.vo \
         $(COQ_DIR)/Tactics.vo $(COQ_DIR)/FindSpec.vo \
         $(COQ_DIR)/InsertDefs.vo $(COQ_DIR)/InsertSpec.vo \
+        $(COQ_DIR)/RebalanceSpec.vo $(COQ_DIR)/InsSpec.vo \
         $(COQ_DIR)/RefCount.vo $(COQ_DIR)/Invariants.vo
 
 # ---- Cleanup ----
